lib/Lib.IntVector.Transpose.fst
@@ -41,7 +41,6 @@ let transpose4x4 #t vs =
   match t with
   | U32 -> transpose4x4_uint32 #t vs
   | U64 -> transpose4x4_uint64 #t vs
-  | _ -> admit()
 
 ///
 ///   transpose8x8
@@ -120,7 +119,6 @@ let transpose8x8 #t vs =
   match t with
   | U32 -> transpose8x8_uint32 #t vs
   | U64 -> transpose8x8_uint64 #t vs
-  | _ -> admit()
 
 ///
 ///  transpose16x16
@@ -250,7 +248,6 @@ let transpose16x16_uint32 #t vs =
 let transpose16x16 #t vs =
   match t with
   | U32 -> transpose16x16_uint32 #t vs
-  | _ -> admit()
 
 
 ///
@@ -631,17 +628,14 @@ let transpose4x4_lemma #t vs =
   match t with
   | U32 -> Classical.forall_intro_2 (transpose4x4_lemma_uint32_ij vs)
   | U64 -> Classical.forall_intro_2 (transpose4x4_lemma_uint64_ij vs)
-  | _ -> admit()
 
 
 let transpose8x8_lemma #t vs =
   match t with
   | U32 -> Classical.forall_intro_2 (transpose8x8_lemma_uint32_ij vs)
   | U64 -> Classical.forall_intro_2 (transpose8x8_lemma_uint64_ij vs)
-  | _ -> admit()
 
 
 let transpose16x16_lemma #t vs =
   match t with
   | U32 -> Classical.forall_intro_2 (transpose16x16_lemma_ij vs)
-  | _ -> admit()
